\documentclass[aps,onecolumn,12pt]{revtex4}
\usepackage{graphicx}
\usepackage{amssymb,amsfonts,amsmath,amsthm}
\usepackage{chemarr}
\usepackage{bm}
\usepackage{pslatex}
\usepackage{xfrac}
\usepackage[dvipsnames]{xcolor}
%\usepackage{bookman}
\usepackage{dsfont}
\usepackage{mathptmx}
\usepackage{hyperref}
%\usepackage{rotating}

\newcommand{\mychem}[1]{\mathtt{#1}}
\newcommand{\myconc}[1]{\left[#1\right]}
\newcommand{\spx}{\mychem{X}}
\newcommand{\spproton}{\mychem{H^+}}
\newcommand{\proton}{\myconc{\spproton}}


\begin{document}
%\large
\title{Cooperativity}
\maketitle

\section{One Layer}

\subsection{Scheme}
\begin{equation}
\boxed{
\begin{array}{ccccc}
 & & E_{01}  &  & \\
 &  \rotatebox{45}{$+\spx_1^{out}\xrightleftharpoons[d_{01}]{a_{01}C_1}$} &   & \rotatebox{-45}{$\xrightarrow[-\spx_1^{in}]{+ \spproton, \; k^p_1}$} &  \\
E_{00}  &  & \xleftarrow{\text{recycling  by } k_h } &   & E_{0H} \\
  & \rotatebox{-45}{$+\spx_2^{out}\xrightleftharpoons[d_{02}]{a_{02}C_2}$} &   & \rotatebox{+45}{$\xrightarrow[-\spx_2^{in}]{+ \spproton, \; k^p_2}$} & \\
 & & E_{02} & & \\
 \end{array}
 }
\end{equation}

\subsection{Equations}

\begin{equation}
\left\lbrace
\begin{array}{rcl}
\partial_t E_{00} & = & D_{01}-A_{01} + D_{02}-A_{02} + v_h\\
\partial_t E_{01} & = & -D_{01}+A_{01} -v^p_1 \\
\partial_t E_{02} & = & -D_{02}+A_{02} -v^p_2\\
\partial_t E_{0H} & = & v^p_1 + v^p_2 - v_h\\
\mathcal{E}       & = & E_{00}+E_{01}+E_{02} + E_{0H} = E_{0H} + {\displaystyle \sum_{x\leq y\leq 1} E_{xy}}\\
\end{array}
\right.
\end{equation}
with
\begin{equation}
\left\lbrace
\begin{array}{rcl}
C_1    & = & \myconc{\spx_1^{out}}\\
C_2    & = & \myconc{\spx_2^{out}}\\
A_{01} &= &a_{01} E_{00} C_1\\
A_{02} &= &a_{02} E_{00} C_2\\
D_{01} &= &d_{01} E_{01}\\
D_{02} &= &d_{02} E_{02}\\
v^p_1  &=& k^p_1 E_{01} \proton\\
v^p_2  &=& k^p_2 E_{02} \proton\\
v_h    &=& k_x  E_{0H}
\end{array}
\right.
\end{equation}

\subsection{Steady-State}
\subsubsection{Raw Equations}
We assume that the internal components are at a steady-state:
\begin{equation}
\left\lbrace
\begin{array}{rcll}
	E_{01}^\star & = & \dfrac{a_{01}}{d_{01}+k^p_1 \proton } E_{00} C_1 & = J_1 E_{00} C_1\\
	\\
	E_{02}^\star & = & \dfrac{a_{02}}{d_{02}+k^p_2 \proton } E_{00} C_2 & = J_2 E_{00} C_2\\
\end{array}
\right.
\end{equation}
We expect a simplification if $d_{01},d_{02} \gg k^p_1 \proton, k^p_2 \proton$.
Finally:
\begin{equation}
\mathcal{E} = E_{00}\left[1+J_1C_1+J_2C_2\right] + E_{0H} \Leftrightarrow E_{00} = \dfrac{\mathcal{E}-E_{0H}}{\underbrace{1+J_1C_1+J_2C_2}_{\mathfrak{D}}}
\end{equation}
and:
\begin{equation}
\left\lbrace
\begin{array}{rcl}
	E_{01}^\star & = & \dfrac{J_1C_1}{1+J_1C_1+J_2C_2} \left(\mathcal{E}-E_{0H}\right)\\
	\\
	E_{02}^\star & = & \dfrac{J_2C_2}{1+J_1C_1+J_2C_2} \left(\mathcal{E}-E_{0H}\right)
\end{array}
\right.
\end{equation}
so that we have the three equations:
\begin{equation}
\left\lbrace
\begin{array}{rcl}
	\partial_t \myconc{X_u}_{in} & = & \dfrac{k^p_u J_uC_u}{1+J_1C_1+J_2C_2} \left(\mathcal{E}-E_{0H}\right) \proton + \text{other sources...} \\
	\\
	\partial_t E_{0H} & = & -k_h E_{0H} + \dfrac{k^p_1 J_1C_1 + k^p_2 J_2 C_2 }{1+J_1C_1+J_2C_2} \left(\mathcal{E}-E_{0H}\right) \proton \\
\end{array}
\right.
\end{equation}
\subsubsection{Normalisation}


\section{Two Layers}

\begin{equation}
\boxed{
\begin{array}{ccccc}
 & & E_{01} & \xrightleftharpoons[d_{11}]{a_{11}C_1} & E_{11}\\
 &  \rotatebox{45}{$\xrightleftharpoons[d_{01}]{a_{01}C_1}$} &   & \rotatebox{-45}{$\xrightleftharpoons[d_{12}]{a_{12}C_2}$} & \\
E_{00} & &  & & E_{12}\\ 
  & \rotatebox{-45}{$\xrightleftharpoons[d_{02}]{a_{02}C_2}$} &  & \rotatebox{45}{$\xrightleftharpoons[d_{21}]{a_{21}C_1}$} &  \\
  & & E_{02} & \xrightleftharpoons[d_{22}]{a_{22}C_2} & E_{22}\\
 \end{array}
 }
\end{equation}


\begin{equation}
\left\lbrace
\begin{array}{rcl}
\partial_t E_{00} & = & D_{01}-A_{01} + D_{02}-A_{02}\\
\partial_t E_{01} & = & -D_{01}+A_{01} - A_{11} + D_{11} - A_{12} + D_{12}\\
\partial_t E_{02} & = & -D_{02}+A_{02} - A_{22} + D_{22} - A_{21} + D_{21}\\
\partial_t E_{11} & = & A_{11}-D_{11}\\
\partial_t E_{12} & = & A_{12}-D_{12} + A_{21}-D_{21}\\
\partial_t E_{22} & = & A_{22}-D_{22}\\
\mathcal{E}       & = & {\displaystyle \sum_{x\leq y\leq 2} E_{xy}}\\
\end{array}
\right.
\end{equation}
with
\begin{equation}
\left\lbrace
\begin{array}{rcl}
A_{01} &= &a_{01} E_{00} C_1\\
A_{02} &= &a_{02} E_{00} C_2\\
D_{01} &= &d_{01} E_{01}\\
D_{02} &= &d_{02} E_{02}\\
A_{11} &= & a_{11} E_{01} C_1 \\
D_{11} &= &d_{11} E_{11}\\
A_{22} &= &a_{22} E_{02} C_2 \\
D_{22} &= &d_{22} E_{22}\\
A_{12} & = & a_{12} E_{01} C_2\\
D_{12} & = & d_{12} E_{12}\\
A_{21} & = & a_{21} E_{02} C_1\\
D_{21} & = & d_{21} E_{12}\\
\end{array}
\right.
\end{equation}
The second layer yields:
\begin{equation}
\left\lbrace
\begin{array}{rcl}
0 & = & A_{11}^\star-D_{11}^\star\\
0 & = & A_{12}^\star-D_{12}^\star + A_{21}^\star-D_{21}^\star\\
0 & = & A_{22}^\star-D_{22}^\star\\
\end{array}
\right.
\end{equation}
or

\begin{equation}
\left\lbrace
\begin{array}{rcl}
0 & = & a_{11} E_{01}^\star C_1 - d_{11} E_{11}^\star\\
0 & = & a_{12} E_{01}^\star C_2  + a_{21} E_{02}^\star C_1 - \left(d_{12}+d_{21}\right) E_{12}^\star\\
0 & = & a_{22} E_{02}^\star C_2 -d_{22} E_{22}^\star\\
\end{array}
\right.
\end{equation}
so that
\begin{equation}
\left\lbrace
\begin{array}{rcl|l}
	E_{11}^\star & = & k_{11} E_{01}^\star C_1 & k_{11} = \dfrac{a_{11}}{d_{11}}\\
	 & & & \\
	E_{22}^\star & = & k_{22} E_{02}^\star C_2 & k_{22} = \dfrac{a_{22}}{d_{22}}\\
	 & & & \\
	E_{12}^\star & = & k_{12} E_{01}^\star C_2 + k_{21} E_{02}^\star C_1  & k_{12} = \dfrac{a_{12}}{d_{12}+d_{21}},\; k_{21} = \dfrac{a_{21}}{d_{12}+d_{21}} \\
\end{array}
\right.
\end{equation}
We are left with the (redundant) first layer equations
\begin{equation}
\left\lbrace
\begin{array}{rcl}
0 & = & D_{01}^\star-A_{01}^\star + D_{02}^\star-A_{02}^\star\\
0 & = & -D_{01}^\star+A_{01}^\star  - A_{12}^\star + D_{12}^\star\\
0 & = & -D_{02}^\star+A_{02}^\star  - A_{21}^\star + D_{21}^\star\\
\end{array}
\right.
\end{equation}
leading to
\begin{equation}
\left\lbrace
\begin{array}{rcl}
d_{01}E_{01}^\star + d_{02} E_{02}^\star & = & \left( a_{01}C_1+a_{02}C_2\right)E_{00}^\star\\
A_{01}^\star & = & A_{12}^\star + D_{01}^\star - D_{12}^\star\\
A_{02}^\star & = & A_{21}^\star + D_{02}^\star - D_{21}^\star\\ 
\end{array}
\right.
\end{equation}
or
\begin{equation}
\left\lbrace
\begin{array}{rcl}
d_{01}E_{01}^\star + d_{02} E_{02}^\star & = & \left( a_{01}C_1+a_{02}C_2\right)E_{00}^\star\\
a_{01} E_{00}^\star C_1 & = & a_{12} E_{01}^\star C_2  + d_{01}E_{01}^\star - d_{12}E_{12}^\star\\
a_{02} E_{00}^\star C_2 & = & a_{21}E_{02}^\star C_1 + d_{02}E_{02}^\star - d_{21}E_{12}^\star\\ 
\end{array}
\right.
\end{equation}

\begin{equation}
\left\lbrace
\begin{array}{rcl}
a_{01} E_{00}^\star C_1 & = & a_{12} E_{01}^\star C_2  + d_{01}E_{01}^\star - d_{12}\left( k_{12} E_{01}^\star C_2 + k_{21} E_{02}^\star C_1 \right)\\
a_{02} E_{00}^\star C_2 & = & a_{21}E_{02}^\star C_1 + d_{02}E_{02}^\star - d_{21} \left( k_{12} E_{01}^\star C_2 + k_{21} E_{02}^\star C_1 \right)\\ 
\end{array}
\right.
\end{equation}



\end{document}
